remove a sorry in Vector.getElem_zipWith3

Projects/Wuethrich/Vector.lean
@@ -1,8 +1,6 @@
 import Projects.Wuethrich.Array
 import Projects.Wuethrich.Aux
 
-section Vector
-
 variable {α : Type} {n : ℕ}
 
 def Vector.restrictEven (xs : Vector α (2 ^ (n + 1))) : Vector α (2 ^ n) :=
@@ -21,17 +19,25 @@ lemma restrictOdd_of_vector {xs : Vector α (2 ^ (n + 1))} :
   funext j
   simp [restrictOdd, Fin.doubleSucc, Vector.restrictOdd]
 
-def Vector.zipWith3 {α β γ δ : Type*} {n : ℕ} (f : α → β → γ → δ)
+
+
+namespace Vector
+
+def zipWith3 {α β γ δ : Type*} {n : ℕ} (f : α → β → γ → δ)
     (v1 : Vector α n) (v2 : Vector β n) (v3 : Vector γ n) : Vector δ n :=
   ⟨Array.zipWith3 f v1.toArray v2.toArray v3.toArray, by simp⟩
   --Vector.ofFn (fun i => f (v1.get i) (v2.get i) (v3.get i))
 
-@[simp, grind =] theorem Vector.getElem_zipWith3 {α β γ δ : Type*} {f : α → β → γ → δ} {as : Vector α n} {bs : Vector β n} {cs : Vector γ n} {i : Nat}
+variable {α β γ δ : Type*}
+
+@[simp] theorem mk_zipWith3_mk {f : α → β → γ → δ} {as : Array α} {bs : Array β} {cs : Array γ}
+    (h : as.size = n) (h' : bs.size = n) (h'' : cs.size = n) :
+    Vector.zipWith3 f (Vector.mk as h) (Vector.mk bs h') (Vector.mk cs h'') =
+      Vector.mk (Array.zipWith3 f as bs cs) (by simp [h, h', h'']) := rfl
+
+@[simp, grind =] theorem getElem_zipWith3  {f : α → β → γ → δ} {as : Vector α n} {bs : Vector β n} {cs : Vector γ n} {i : Nat}
     (hi : i < n) : (Vector.zipWith3 f as bs cs)[i] = f as[i] bs[i] cs[i] := by
   cases as
   cases bs
   cases cs
   simp
-  sorry
-
-end Vector
